Verity/Macro/Syntax.lean
@@ -55,7 +55,13 @@ syntax "initializer(" ident ")" : verityInitGuard
 syntax "reinitializer(" ident ", " num ")" : verityInitGuard
 syntax "ecmCall " term:max ppSpace term:max : term
 syntax "ecmDo " term:max ppSpace term:max : term
+syntax "adt " str : term
+syntax "adt " str " [" sepBy(term, ",") "]" : term
 syntax "tryCatch " term:max ppSpace term:max : doElem
+
+macro_rules
+  | `(adt $_variant:str) => `(0)
+  | `(adt $_variant:str [ $[$_args:term],* ]) => `(0)
 syntax "revert " ident "(" sepBy(term, ",") ")" : doElem
 syntax "revertError " ident "(" sepBy(term, ",") ")" : doElem
 syntax "requireError " term:max ppSpace ident "(" sepBy(term, ",") ")" : doElem
